A lot of changes

examples/bytestring/main.c
@@ -1,0 +1,20 @@
+#include <stdio.h>
+#include <stdlib.h>
+#include "gc.h"
+
+extern value body(struct thread_info *);
+extern void print_Coq_Init_Datatypes_nat(int_or_ptr64);
+
+_Bool is_ptr(unsigned int s) {
+  return (_Bool) Is_block(s);
+} 
+
+int main(int argc, char *argv[]) {
+  struct thread_info* tinfo;
+
+  tinfo = make_tinfo();
+  body(tinfo);
+
+  puts("");
+  return 0;
+}
