examples/bytestring/prims.h
@@ -1,0 +1,3 @@
+value nat_to_ull(value);
+value runM(struct thread_info *tinfo, value, value);
+value array_runM(struct thread_info *tinfo, value, value, value, value);
