generator/Desc.v
@@ -18,7 +18,7 @@ Require Import VeriFFI.library.meta.
 Require Import VeriFFI.generator.GraphPredicate.
 Require Import VeriFFI.generator.InGraph.
 
-(*Unset Strict Unquote Universe Mode.*) (* There is no flag or option with this name *)
+(* Unset MetaCoq Strict Unquote Universe Mode. *)
 
 (* Require Import VeriFFI.generator.InGraph. *)
 (* MetaCoq Run (in_graph_gen bool). *)
@@ -33,6 +33,9 @@ Require Import VeriFFI.generator.InGraph.
 Import monad_utils.MCMonadNotation
        ListNotations
        MetaCoqNotations.
+
+Set Universe Polymorphism.
+(* Set Polymorphic Inductive Cumulativity. *)
 
 Fixpoint adjust_context (ctx : list (Kernames.ident * Reppyish)) : TemplateMonad (list (Kernames.ident * named_term)) :=
   match ctx with
@@ -65,14 +68,28 @@ Definition fill_hole
   tmEval all quantified >>= tmPrint ;;
   hoisted <- instance_term quantified ;;
   (* make function application again to have the same free variables *)
-  ret (tApp hoisted (rev (map (fun '(id, _) => tVar id) named_ctx))).
+  tmMsg! "hole ctx:" ;;
+  tmEval all named_ctx >>= tmPrint! ;;
+  let ctx_to_apps : list named_term :=
+    rev (map (fun '(id, t) =>
+                match t with
+                | tApp (tInd {| inductive_mind := kn; inductive_ind := 0 |} _) _ =>
+                    if eq_kername kn <? InGraph ?>
+                    then tApp <% @field_in_graph %> [hole; tVar id]
+                    (* then tApp (tConst (MPfile ["meta"; "library"; "VeriFFI"], "field_in_graph") []) [hole; tVar id] *)
+                    else tVar id
+                | _ => tVar id
+                end) named_ctx) in
+  ret (tApp hoisted ctx_to_apps).
+  (* ret (strip_lambdas hoisted). *)
+  (* ret (tApp hoisted (rev (map (fun '(id, _) => tVar id) named_ctx))). *)
 
 (*
 MetaCoq Run (fill_hole [("H", tApp <% InGraph %> [tVar "a"]);("a", <% Type %>)]
                        (tApp <% InGraph %> [tApp <% @list %> [tVar "a"]]) >>= tmEval all >>= tmPrint).
 *)
 
-Definition create_reific
+Polymorphic Definition create_reific
            (ind : inductive)
            (mut : mutual_inductive_body)
            (one : one_inductive_body)
@@ -104,7 +121,7 @@ Definition create_reific
             | nNamed id => (h, tApp <% @InGraph %> [tVar id]) :: (id, t) :: named_ctx
             | _ => named_ctx end in
         rest <- go b index_ctx named_ctx' (pred num_params) ;;
-        let f := tLambda n (tSort s) (tLambda H (tApp <% @InGraph %> [tRel O]) rest) in
+        let f := tLambda n (tSort s) (tLambda H (tApp <% @ctor_ann %> [tRel O]) rest) in
         ret (tApp <% @TYPEPARAM ctor_ann %> [f])
 
       | tProd n t b , O =>
@@ -129,8 +146,8 @@ Definition create_reific
 
   let num_of_params := ind_npars mut in
   c <- go t' init_index_ctx [] num_of_params ;;
-  (* tmMsg "after go:" ;; *)
-  (* tmEval all c >>= tmPrint ;; *)
+  tmMsg "after go:" ;;
+  tmEval all c >>= tmPrint! ;;
   c' <- DB.deBruijn c ;;
   (* tmMsg "after de bruijn:" ;; *)
   (* tmEval all c' >>= tmPrint ;; *)
@@ -173,46 +190,80 @@ Definition desc_gen {T : Type} (ctor_val : T) : TemplateMonad unit :=
   | t' => tmPrint t' ;; tmFail "Not a constructor"
   end.
 
-(* Definition descs_gen {kind : Type} (Tau : kind) : TemplateMonad unit := *)
-(*   '(env, tau) <- tmQuoteRec Tau ;; *)
-(*   match declarations (env) with *)
-(*   | (kn, InductiveDecl decl) :: _ => *)
-(*     let each_ctor (mut_type_count : nat) *)
-(*                   (ctor_count : nat) *)
-(*                   (ctor : constructor_body) : TemplateMonad unit := *)
-(*       t <- tmUnquote (tConstruct {| inductive_mind := kn *)
-(*                                   ; inductive_ind := mut_type_count |} *)
-(*                                 ctor_count []) ;; *)
-(*       t' <- tmEval all (my_projT2 t) ;; *)
-(*       (* ty_t' <- tmEval all (my_projT1 t) ;; *) *)
-(*       (* let '(ctor_name, _, _) := ctor in *) *)
-(*       (* @desc_gen _ t' ctor_name *) *)
-(*       @desc_gen _ t' *)
-(*     in *)
-(*     let all_in_one (mut_type_count : nat) *)
-(*                   (one : one_inductive_body) : TemplateMonad unit := *)
-(*       let ctors := ind_ctors one in *)
-(*       monad_map_i (each_ctor mut_type_count) (ind_ctors one) ;; ret tt *)
-(*     in *)
-(*     let all_in_mut (mut : mutual_inductive_body) : TemplateMonad unit := *)
-(*       monad_map_i all_in_one (ind_bodies mut) ;; ret tt *)
-(*     in *)
-(*     all_in_mut decl *)
-(*   | _ => tmFail "Need an inductive type in the environment" *)
-(*   end. *)
+Definition descs_gen {kind : Type} (Tau : kind) : TemplateMonad unit :=
+  '(env, tau) <- tmQuoteRec Tau ;;
+  match declarations (env) with
+  | (kn, InductiveDecl decl) :: _ =>
+    let each_ctor (mut : mutual_inductive_body)
+                  (one : one_inductive_body)
+                  (mut_type_count : nat)
+                  (ctor_count : nat)
+                  (ctor : constructor_body) : TemplateMonad unit :=
+      let ind := {| inductive_mind := kn ; inductive_ind := mut_type_count |} in
+      t <- tmUnquote (tConstruct ind ctor_count []) ;;
+      let '{| my_projT1 := T; my_projT2 := ctor_val |} := t in
+
+      reific <- create_reific ind mut one ctor ;;
+      (* tmPrint "after create reific" ;; *)
+      (* tmEval all reific >>= tmPrint ;; *)
+
+      newName <- tmFreshName "new"%bs ;;
+      reflected <- tmLemma newName (@reflector ctor_ann T ctor_val reific) ;;
+
+      let d := {| ctor_name := cstr_name ctor
+                ; ctor_reified := reific
+                ; ctor_reflected := reflected
+                ; ctor_tag := ctor_count
+                ; ctor_arity := cstr_arity ctor
+                |} in
+
+      name <- tmFreshName (cstr_name ctor ++ "_desc")%bs ;;
+      @tmDefinition name (@Desc T ctor_val) {| desc := d |} ;;
+      (* Declare the new definition a type class instance *)
+      mp <- tmCurrentModPath tt ;;
+      tmExistingInstance (ConstRef (mp, name)) ;;
+      ret tt
+
+    in
+    let all_in_one (mut : mutual_inductive_body)
+                   (mut_type_count : nat)
+                   (one : one_inductive_body) : TemplateMonad unit :=
+      let ctors := ind_ctors one in
+      monad_map_i (each_ctor mut one mut_type_count) (ind_ctors one) ;; ret tt
+    in
+    let all_in_mut (mut : mutual_inductive_body) : TemplateMonad unit :=
+      monad_map_i (all_in_one mut) (ind_bodies mut) ;; ret tt
+    in
+    all_in_mut decl
+  | _ => tmFail "Need an inductive type in the environment"
+  end.
 
 Obligation Tactic := reflecting.
 
-(* Ltac gen := *)
-(*   match goal with *)
-(*   | [ |- @reflector _ _ _ _ ] => reflecting *)
-(*   | _ => in_graph_gen_tac *)
-(*   end. *)
+Ltac gen :=
+  match goal with
+  | [ |- @reflector _ _ _ _ ] => reflecting
+  | _ => in_graph_gen_tac
+  end.
 
-(* Obligation Tactic := gen. *)
+Obligation Tactic := gen.
+
+Unset MetaCoq Strict Unquote Universe Mode.
+
+(* Set Universe Polymorphism. *)
+(* Set Polymorphic Inductive Cumulativity. *)
+
+(* MetaCoq Run (in_graph_gen option). *)
+(* MetaCoq Run (descs_gen option). *)
+(* MetaCoq Run (@desc_gen _ (@None)). *)
 
 (* MetaCoq Run (in_graph_gen unit). *)
+(* MetaCoq Run (descs_gen unit). *)
+
 (* MetaCoq Run (in_graph_gen nat). *)
+(* MetaCoq Run (descs_gen nat). *)
+
+
 (* MetaCoq Run (desc_gen tt). *)
 (* MetaCoq Run (desc_gen S). *)
 (* Set Printing All. *)
