generator/funspec.v
@@ -1,0 +1,93 @@
+Require Import String.
+
+Require Import ZArith.
+Require Import Psatz.
+Require Import List.
+Import ListNotations.
+
+Require Import VeriFFI.library.isomorphism.
+Require Import VeriFFI.library.meta.
+Require Import VeriFFI.library.modelled.
+
+Require Import VeriFFI.verification.graph_add.
+Require Import VeriFFI.verification.specs_library.
+Require Import VeriFFI.verification.specs_general.
+
+Require Import VST.floyd.proofauto.
+
+Definition tvalue : type :=
+  talignas (if Archi.ptr64 then 3%N else 2%N) (tptr tvoid).
+
+Definition t_tinfo : type := Tstruct (ident_of_string "thread_info") noattr.
+
+Definition get_c_typesig
+           (c : reified prim_ann)
+           (arity : nat) : compcert_rmaps.typesig :=
+  (cons t_tinfo (repeat tvalue arity), tvalue).
+
+(** Generation of the in_graph predicates, given the constructor arguments. *)
+Fixpoint in_graphs
+         (g : graph) (c : reified prim_ann) (xs : args c) (ps : list rep_type) : Prop :=
+  match c as l return (args l -> Prop) with
+  | TYPEPARAM f =>
+      fun H =>
+        let '(A; (ann; xs')) := H in
+        in_graphs g (f A ann) xs' ps
+  | ARG A ann f =>
+      fun H =>
+        let '(x; xs') := H in
+        match ps with
+        | [] => False
+        | p :: ps' => @is_in_graph A (@prim_in_graph A ann) g x p /\ in_graphs g (f x) xs' ps'
+        end
+  | RES x _ => fun _ => ps = nil
+  end xs.
+
+Definition ep_to_funspec_aux
+           (c : reified prim_ann)
+           (uncurried_model_fn : meta.reflect c)
+           (arity : nat) : funspec :=
+  NDmk_funspec
+    (get_c_typesig c arity)
+    cc_default
+    (globals * graph * GCGraph.roots_t * share * args c * list rep_type *
+       val * GCGraph.outlier_t * GCGraph.fun_info * GCGraph.thread_info)
+    (fun x => match x with
+     | (gv, g, roots, sh, xs, ps, ti, outlier, f_info, t_info) =>
+       PROP (writable_share sh ;
+              in_graphs g c xs ps)
+       (PARAMSx (ti :: map (rep_type_val g) ps)
+       (SEPx (full_gc g t_info roots outlier ti sh :: nil)))
+     end)
+    (fun x => match x with
+     | (gv, g, roots, sh, xs, ps, ti, outlier, f_info, t_info) =>
+       EX (p' : rep_type) (g' : graph) (t_info' : GCGraph.thread_info),
+          PROP (let r := result c xs in
+                @is_in_graph (projT1 r) (@prim_in_graph (projT1 r) (projT2 r)) g'
+                  (uncurried_model_fn xs) p' ;
+                gc_graph_iso g roots g' roots)
+          RETURN  (rep_type_val g' p')
+          SEP (full_gc g' t_info' roots outlier ti sh)
+     end).
+
+Definition ep_to_funspec (d : fn_desc) (xs : args (type_desc d)) : ident * funspec :=
+  (ident_of_string (c_name d),
+   ep_to_funspec_aux (type_desc d) (uncurried_model_fn d) (f_arity d)).
+
+(* Definition uint63_to_nat_spec :  funspec :=  *)
+(*    WITH gv : globals, g : graph, roots : roots_t, sh : share, n: nat, *)
+(*         ti : val, outlier : outlier_t, f_info : fun_info, t_info : GCGraph.thread_info *)
+(*    PRE  [ tptr t_tinfo,  (talignas 3%N (tptr tvoid)) ] *)
+(*       PROP ( (Z.of_nat n) < headroom t_info ; (* KS: 2 times this *) *)
+(*             writable_share sh  *)
+(*             (* min_signed <= encode_Z (Z.of_nat n) <= max_signed *) *)
+(*             ) *)
+(*       (PARAMSx [ti; Vlong (Int64.repr (encode_Z (Z.of_nat n)))] *)
+(*       (GLOBALSx nil *)
+(*       (SEPx (full_gc g t_info roots outlier ti sh :: nil)))) *)
+(*    POST [ (talignas 3%N (tptr tvoid)) ] *)
+(*      EX (p' : rep_type) (g' : graph) (t_info' : GCGraph.thread_info), *)
+(*        PROP (@is_in_graph nat (@in_graph nat _) g' n p' ; *)
+(*              gc_graph_iso g roots g' roots) *)
+(*        RETURN  (rep_type_val g' p') *)
+(*        SEP (full_gc g' t_info' roots outlier ti sh) . *)
