tests/generators.v
@@ -1,0 +1,101 @@
+(*
+Require Import VeriFFI.generator.Rep.
+
+MetaCoq Run (gen_for unit).
+MetaCoq Run (gen_for bool).
+MetaCoq Run (gen_for nat).
+MetaCoq Run (gen_for option).
+MetaCoq Run (gen_for prod).
+MetaCoq Run (gen_for list).
+
+Inductive vec (A : Type) : nat -> Type :=
+| vnil : vec A O
+| vcons : forall n, A -> vec A n -> vec A (S n).
+
+MetaCoq Run (gen_for nat).
+
+Inductive option_indexed : Type -> Type :=
+| mysome : forall A, A -> option_indexed A.
+(* This is supposed to fail because if the type argument is not a parameter,
+   then knowing how to represent things of that type statically is tricky,
+   and often impossible. *)
+Fail MetaCoq Run (gen_for option_indexed).
+
+Inductive mylist (A B : Type) : Type :=
+| mynil : mylist A B
+| mycons : A -> option A -> option B -> mylist A B.
+MetaCoq Run (in_graph_gen mylist).
+
+(* Testing mutually recursive inductive types: *)
+Inductive T1 :=
+| c1 : T2 -> T1
+with T2 :=
+| c2 : T1 -> T2.
+MetaCoq Run (gen_for T1).
+
+Inductive tree (A : Type) : Type :=
+| tleaf : tree A
+| tnode : nat -> forest A -> tree A
+with forest (A : Type) : Type :=
+| fnil : forest A
+| fcons : tree A -> forest A -> forest A.
+MetaCoq Run (gen_for tree)
+
+(* Testing dependent types: *)
+Inductive natty : nat -> nat -> Type :=
+| mynatty : forall n m, natty n m.
+MetaCoq Run (gen_for natty).
+
+Inductive D1 : nat -> Type :=
+| cd1 : forall n : nat, D1 n.
+MetaCoq Run (gen_for D1).
+
+Inductive D2 (n : nat) : Type :=
+| cd2 : D2 n.
+MetaCoq Run (gen_for D2).
+
+Inductive indexed : nat -> Type :=
+| bar : indexed O.
+MetaCoq Run (gen_for indexed).
+
+Inductive fin : nat -> Set :=
+| F1 : forall {n}, fin (S n)
+| FS : forall {n}, fin n -> fin (S n).
+MetaCoq Run (gen_for fin).
+
+Inductive param_and_index (a b : nat) : a < b -> Type :=
+| foo : forall (pf : a < b), param_and_index a b pf.
+MetaCoq Run (gen_for param_and_index).
+
+(* Testing nested types: *)
+(* "Haskell Programming with Nested Types: A Principled Approach", Johann and Ghani, 2009 *)
+Inductive lam (A : Type) : Type :=
+| variable : A -> lam A
+| app : lam A -> lam A -> lam A
+| abs : lam (option A) -> lam A.
+MetaCoq Run (gen_for lam).
+
+Inductive digit (A : Type) : Type :=
+| one : A -> digit A
+| two : A -> A -> digit A
+| three : A -> A -> A -> digit A
+| four : A -> A -> A -> A -> digit A.
+Inductive node (A : Type) : Type :=
+| node2 : nat -> A -> A -> node A
+| node3 : nat -> A -> A -> A -> node A.
+Inductive finger_tree (A : Type) : Type :=
+| emptyT : finger_tree A
+| single : A -> finger_tree A
+| deep : nat -> digit A -> finger_tree (node A) -> digit A -> finger_tree A.
+MetaCoq Run (gen_for finger_tree).
+
+Inductive two (A : Type) :=
+| mkTwo : A -> A -> two A.
+Inductive tree (A : Type) : Type :=
+| leaf : tree A
+| node : two (tree A) -> tree A.
+Inductive ntree (A : Type) : Type :=
+| nleaf : ntree A
+| nnode : ntree (two A) -> ntree A.
+MetaCoq Run (gen_for ntree).
+*)
